change function name

code/experimental/rsapss/Hacl.Spec.Bignum.Convert.fst
@@ -11,50 +11,50 @@ open Hacl.Spec.Bignum
 
 #reset-options "--z3rlimit 50 --max_fuel 0 --max_ifuel 0"
 
-val bignum_from_bytes_be_f: len:size_nat{8 * len <= max_size_t} -> lseq uint8 (8 * len) -> i:nat{i < len} -> uint64
-let bignum_from_bytes_be_f len b i =
+val bn_from_bytes_be_f: len:size_nat{8 * len <= max_size_t} -> lseq uint8 (8 * len) -> i:nat{i < len} -> uint64
+let bn_from_bytes_be_f len b i =
   uint_from_bytes_be (sub b ((len - i - 1) * 8) 8)
 
 
-val bignum_from_bytes_be_: len:size_nat{8 * len <= max_size_t} -> lseq uint8 (8 * len) -> lbignum len
-let bignum_from_bytes_be_ len b = createi len (bignum_from_bytes_be_f len b)
+val bn_from_bytes_be_: len:size_nat{8 * len <= max_size_t} -> lseq uint8 (8 * len) -> lbignum len
+let bn_from_bytes_be_ len b = createi len (bn_from_bytes_be_f len b)
 
 
-val bignum_from_bytes_be: len:size_pos{8 * blocks len 8 <= max_size_t} -> lseq uint8 len -> lbignum (blocks len 8)
-let bignum_from_bytes_be len b =
+val bn_from_bytes_be: len:size_pos{8 * blocks len 8 <= max_size_t} -> lseq uint8 len -> lbignum (blocks len 8)
+let bn_from_bytes_be len b =
   let bnLen = blocks len 8 in
   let tmpLen = 8 * bnLen in
   let tmp = create tmpLen (u8 0) in
   let tmp = update_sub tmp (tmpLen - len) len b in
-  bignum_from_bytes_be_ bnLen tmp
+  bn_from_bytes_be_ bnLen tmp
 
 
-val bignum_to_bytes_be_f: len:size_nat{8 * len <= max_size_t} -> lbignum len -> i:nat{i < len} -> unit -> unit & lseq uint8 8
-let bignum_to_bytes_be_f len b i () =
+val bn_to_bytes_be_f: len:size_nat{8 * len <= max_size_t} -> lbignum len -> i:nat{i < len} -> unit -> unit & lseq uint8 8
+let bn_to_bytes_be_f len b i () =
   (), uint_to_bytes_be b.[len - i - 1]
 
 
-val bignum_to_bytes_be_: len:size_nat{8 * len <= max_size_t} -> lbignum len -> lseq uint8 (8 * len)
-let bignum_to_bytes_be_ len b =
+val bn_to_bytes_be_: len:size_nat{8 * len <= max_size_t} -> lbignum len -> lseq uint8 (8 * len)
+let bn_to_bytes_be_ len b =
   let a_spec (i:nat{i <= len}) = unit in
   let _, o = generate_blocks 8 len len a_spec
-    (bignum_to_bytes_be_f len b) () in
+    (bn_to_bytes_be_f len b) () in
   o
 
 
-val bignum_to_bytes_be: len:size_pos{8 * blocks len 8 <= max_size_t} -> lbignum (blocks len 8) -> lseq uint8 len
-let bignum_to_bytes_be len b =
+val bn_to_bytes_be: len:size_pos{8 * blocks len 8 <= max_size_t} -> lbignum (blocks len 8) -> lseq uint8 len
+let bn_to_bytes_be len b =
   let bnLen = blocks len 8 in
   let tmpLen = 8 * bnLen in
-  let tmp = bignum_to_bytes_be_ bnLen b in
+  let tmp = bn_to_bytes_be_ bnLen b in
   sub tmp (tmpLen - len) len
 
 
-val bignum_from_bytes_be_lemma: len:size_pos{8 * blocks len 8 <= max_size_t} -> b:lseq uint8 len -> Lemma
-  (bn_v (bignum_from_bytes_be len b) == nat_from_bytes_be b)
-let bignum_from_bytes_be_lemma len b = admit()
+val bn_from_bytes_be_lemma: len:size_pos{8 * blocks len 8 <= max_size_t} -> b:lseq uint8 len -> Lemma
+  (bn_v (bn_from_bytes_be len b) == nat_from_bytes_be b)
+let bn_from_bytes_be_lemma len b = admit()
 
 
-val bignum_to_bytes_be_lemma: len:size_pos{8 * blocks len 8 <= max_size_t} -> b:lbignum (blocks len 8){bn_v b < pow2 (8 * len)} -> Lemma
-  (bignum_to_bytes_be len b == nat_to_bytes_be len (bn_v b))
-let bignum_to_bytes_be_lemma len b = admit()
+val bn_to_bytes_be_lemma: len:size_pos{8 * blocks len 8 <= max_size_t} -> b:lbignum (blocks len 8){bn_v b < pow2 (8 * len)} -> Lemma
+  (bn_to_bytes_be len b == nat_to_bytes_be len (bn_v b))
+let bn_to_bytes_be_lemma len b = admit()
