code/experimental/rsapss/Hacl.Impl.RSAPSS.fst
@@ -13,8 +13,6 @@ open Hacl.Impl.MGF
 open Hacl.Bignum.Comparison
 open Hacl.Bignum.Convert
 open Hacl.Bignum.Exponentiation
-open Hacl.Bignum.Addition
-open Hacl.Bignum.Multiplication
 
 module ST = FStar.HyperStack.ST
 module S = Spec.RSAPSS
@@ -276,14 +274,14 @@ let rsapss_sign modBits eBits dBits pLen qLen skey rBlind r2 sLen salt msgLen ms
   pss_encode sLen salt msgLen msg emBits em;
   assume (8 * v (blocks emLen 8ul) <= max_size_t);
   assume (v (blocks emLen 8ul) == v nLen);
-  bignum_from_bytes_be emLen em m;
+  bn_from_bytes_be emLen em m;
   let h = ST.get () in
   mod_exp modBits nLen n r2 m dBits d s;
   assume (8 * v (blocks k 8ul) <= max_size_t);
   assume (v (blocks k 8ul) == v nLen);
   let h1 = ST.get () in
   assume (bn_v h1 s < pow2 (8 * v k));
-  bignum_to_bytes_be k s sgnt;
+  bn_to_bytes_be k s sgnt;
   pop_frame ()
 
 
@@ -325,7 +323,7 @@ let rsapss_verify modBits eBits pkey r2 sLen sgnt msgLen msg =
   let s = create nLen (u64 0) in
   assume (v (blocks k 8ul) == v nLen);
   assume (8 * v (blocks k 8ul) <= max_size_t);
-  bignum_from_bytes_be k sgnt s;
+  bn_from_bytes_be k sgnt s;
 
   let res =
     if (bn_is_less nLen s nLen n) then begin
@@ -334,7 +332,7 @@ let rsapss_verify modBits eBits pkey r2 sLen sgnt msgLen msg =
       assume (v (blocks emLen 8ul) == v nLen);
       let h1 = ST.get () in
       assume (bn_v h1 m < pow2 (8 * v emLen));
-      bignum_to_bytes_be emLen m em;
+      bn_to_bytes_be emLen m em;
       pss_verify sLen msgLen msg emBits em end
     else false in
   pop_frame ();
